add BankSystem class

LoanApplicationProcessing/BankSystem.dfy
@@ -1,13 +1,282 @@
+include "Support.dfy"
+include "Product.dfy"
+include "User.dfy"
+
 module {:extern "BankSystem"} BankSystem
 {
-  import 'Support.dfy.Support'
+  import opened Support
+  import opened Product
+  import opened User
+
   class Bank {
-    // class constants
-    // class variables
-    // class methods
+    
+    // class constants -- N/A
+    
+    // class variables -- not available in Dafny
+    
+    // class methods -- N/A
+    
     // instance constants
+
+    const capitalFundMinimumThreshold: nat := 500_000
+    const referenceAgency: CreditReferenceAgency 
+    
     // instance variables
+
+    var capitalFundValue: nat
+    var reservedFunds: nat 
+    var loans: set<PersonalLoan>                       //    set<Loan>: loans (empty)
+    var customers: set<Customer>                   //    set<Customer>: customers (empty)
+    var customerLoans: map<nat, nat> 
+    
     // constructor
+
+    constructor(aValue: nat, aReferenceAgency: CreditReferenceAgency)
+    ensures this.capitalFundValue == aValue
+    ensures this.referenceAgency == aReferenceAgency
+    {
+      this.capitalFundValue := aValue;
+      this.referenceAgency := aReferenceAgency;
+    }
+    
     // instance methods
+
+    method newApplication(name: string, age: nat, accountNumber: string, sortCode: string, monthlyIncome: real, monthlyOutgoings: real,
+                          requiredAmount: nat, repaymentPeriod: nat) returns ()
+    requires requiredAmount in PersonalLoan.monthLoan24 || requiredAmount in PersonalLoan.monthLoan36 ||
+             requiredAmount in PersonalLoan.monthLoan48 || requiredAmount in PersonalLoan.monthLoan60
+    requires repaymentPeriod == 24 || repaymentPeriod == 36 || repaymentPeriod == 48 || repaymentPeriod == 60                    
+    
+    modifies this`customers
+    modifies this`loans
+    modifies this`customerLoans
+    modifies this`capitalFundValue
+    modifies this`reservedFunds
+    {
+      var interest: real := 0.0;
+      if {
+        case (5_000 <= requiredAmount <= 7_499) => interest := 13.6;
+        case (7_500 <= requiredAmount <= 10_000) => interest := 6.3;
+      }
+      var loan: PersonalLoan? := new PersonalLoan(requiredAmount, repaymentPeriod, interest);
+      var customer: Customer?, applicationStatus: bool := this.registerApplication(name, age, accountNumber, sortCode, monthlyIncome, 
+                                                                                  monthlyOutgoings, loan);
+      if (customer == null || loan == null) {return;}
+      if (customer != null && loan != null) {
+        applicationStatus := this.processApplication(customer, loan);
+      }
+      if {  
+        case applicationStatus == false => loan.setStatus("rejected");
+        case applicationStatus == true => loan.setStatus("approved");
+      }
+      assume !(loan.statusPending == loan.statusRejected == loan.statusApproved);
+      this.completeApplication(customer, loan); 
+    }
+
+    method registerApplication(name: string, age: nat, accountNumber: string, sortCode: string, monthlyIncome: real, monthlyOutgoings: real, 
+                               aLoan: PersonalLoan) returns (aCustomer: Customer, isLoanRegistered: bool)
+    modifies this`customers
+    modifies this`loans
+    modifies this`customerLoans
+    modifies aLoan`statusPending
+    modifies aLoan`statusRejected
+    modifies aLoan`statusApproved
+    modifies this`capitalFundValue
+    modifies this`reservedFunds
+    {
+      var customer: Customer? := this.registerCustomer(name, age, accountNumber, sortCode, monthlyIncome, monthlyOutgoings); 
+      var loanRegistered: bool := this.registerLoan(aLoan);
+      if (customer != null) {
+        var customerRef: nat := customer.getCustomerReference();
+        var loanRef: nat := aLoan.getLoanReference();
+        this.associateCustomerLoan(loanRef, customerRef);
+        var message: string := "Your application has been recieved and will be processed";
+        this.informCustomer(customer, message);
+      } 
+      return customer, loanRegistered;
+    }
+
+    method registerCustomer(name: string, age: nat, accountNumber: string, sortCode: string, monthlyIncome: real, monthlyOutgoings: real) returns (newCustomer: Customer)
+    modifies this`customers
+    {
+      var aCustomer: Customer? := new Customer(name, age, accountNumber, sortCode, monthlyIncome, monthlyOutgoings);
+      if (aCustomer != null) {this.addCustomer(aCustomer);}
+      return aCustomer;
+    }
+    
+    method registerLoan(aLoan: PersonalLoan) returns (success: bool)
+    modifies this`capitalFundValue
+    modifies this`reservedFunds
+    modifies this`loans
+    modifies aLoan`statusPending
+    modifies aLoan`statusRejected
+    modifies aLoan`statusApproved
+    {
+      var verified: bool := false;
+      var loanAmount: nat := aLoan.getRequiredAmount();
+      verified := this.verifyCapitalAmount(this.capitalFundValue, this.capitalFundMinimumThreshold, loanAmount); // verify capital fund
+        // insert logging message cpital amount
+      if (verified) {verified := this.reserveLoanFunds(aLoan);} // capital amount has been verified so reserve loan funds
+      // insert logging message reserved loan funds
+      if (verified) {this.addLoan(aLoan);} // loan funds have been reserved so add loan to collection of loans
+      if (!verified) {
+        aLoan.setStatus("rejected"); // capital fund or reserve loan fund verification has failed
+        // customer is informed in this.completeApplication()
+      }
+      return verified;
+    }
+
+    method associateCustomerLoan(loanReferenceNumber: nat, customerReferenceNumber: nat) returns ()
+    modifies this`customerLoans
+    ensures loanReferenceNumber in customerLoans
+    ensures customerLoans[loanReferenceNumber] == customerReferenceNumber
+    {
+      this.customerLoans := map[loanReferenceNumber := customerReferenceNumber];
+    }
+
+    method processApplication(aCustomer: Customer, aLoan: PersonalLoan) returns (isSuccessful: bool)
+    {
+      var verified: bool := false;
+      var customerAge: nat := aCustomer.getAge();
+      verified := aLoan.verifyAgeCriteria(customerAge);
+      if (!verified) {
+        var message: string := "Your application has failed the loan age criteria process";
+        this.informCustomer(aCustomer, message);
+        return verified;
+      }
+      var customerMonthlyIncome: real := aCustomer.getMonthlyIncome();
+      var customerMonthlyOutgoings : real := aCustomer.getMonthlyOutgoings();
+      verified := aLoan.verifyIncomeCriteria(customerMonthlyIncome, customerMonthlyOutgoings);
+      if (!verified) {
+        var message: string := "Your application has failed the loan income criteria process";
+        this.informCustomer(aCustomer, message);
+        return verified;
+      }
+      var customerCreditScore: nat := this.obtainCustomerCreditScore(this.referenceAgency, aCustomer);
+      verified := aLoan.verifyCreditScore(customerCreditScore);
+      if (!verified) {
+        var message: string := "Your application has failed the credit score criteria process";
+        this.informCustomer(aCustomer, message);
+        return verified;
+      }
+      return verified;
+    }
+
+    method addLoan(aLoan: PersonalLoan) returns ()
+    modifies this`loans
+    ensures aLoan in this.loans
+    {
+      this.loans := this.loans + {aLoan};      // union of the two sets
+    }
+
+    method addCustomer(aCustomer: Customer) returns ()
+    modifies this`customers
+    ensures aCustomer in this.customers
+    {
+      this.customers := this.customers + {aCustomer};
+    }
+
+    method informCustomer(aCustomer: Customer, message: string) returns ()
+    {
+      var customerName := aCustomer.getName();
+      var customerMessage := "Customer Message: " + customerName + " :: " + message;
+      print customerMessage, "\n"; 
+    }
+
+    method obtainCustomerCreditScore(referenceAgency: CreditReferenceAgency, aCustomer: Customer) returns (score: nat)
+    {
+      var customerName: string := aCustomer.getName();
+      assume customerName in referenceAgency.creditScores;
+      var aScore: nat := referenceAgency.getCreditScore(customerName); 
+      return aScore;
+    }
+
+    method verifyCapitalAmount(fundValue: nat, fundMinimum: nat, loanAmount: nat) returns (isVerified: bool)
+    ensures isVerified == ((fundValue - loanAmount) >= fundMinimum)
+    ensures !isVerified == ((fundValue - loanAmount) < fundMinimum) 
+    {
+      return ((fundValue - loanAmount) >= fundMinimum);
+    }
+
+    method reserveLoanFunds(theLoan: PersonalLoan) returns (success: bool)
+    modifies this`capitalFundValue
+    modifies this`reservedFunds
+    ensures (this.capitalFundValue + this.reservedFunds) == (old(capitalFundValue) + old(reservedFunds)) 
+    {
+      var loanAmount: nat := theLoan.getRequiredAmount();
+      var startingCapitalfund: nat := this.capitalFundValue;
+      var startingReserveFund: nat := this.reservedFunds;
+      assume (this.capitalFundValue - loanAmount) > 0;  
+      this.capitalFundValue := this.capitalFundValue - loanAmount;
+      this.reservedFunds := this.reservedFunds + loanAmount;
+      var finishingCapitalFund: nat := this.capitalFundValue;
+      var finishingReservedFund: nat := this.reservedFunds;
+      var both: bool := (finishingCapitalFund == (startingCapitalfund - loanAmount)) && 
+                        (finishingReservedFund == (startingReserveFund + loanAmount));
+      return both;
+    }
+
+    method completeApplication(theCustomer: Customer, theLoan: PersonalLoan) returns ()
+    requires !(theLoan.statusPending == theLoan.statusRejected == theLoan.statusApproved)
+    modifies this`capitalFundValue
+    modifies this`reservedFunds
+    {
+      var loanStatus: string := theLoan.getStatus();
+      if (loanStatus == "rejected") {
+        var message: string := "We are sorry that your application cannot be processed at this time.";
+        var fundsReleased: bool := this.releaseLoanFunds(theLoan);
+        if (fundsReleased) {
+          // add logging
+          var message: string := "Loan funds released";
+          this.logEvent(message);
+        }
+      }
+      if (loanStatus == "approved") {
+        var success: bool := transferLoanToCustomer(theLoan, theCustomer);
+        var accNo: string, sortCode: string := theCustomer.getPaymentDetails();
+        var message: string := "Your application has been successful. The required loan amount has been transferred to account number: " + 
+                                accNo + " sort code: " + sortCode;
+        this.informCustomer(theCustomer, message);
+      }
+    }
+
+    method releaseLoanFunds(theLoan: PersonalLoan) returns (success: bool)
+    modifies this`capitalFundValue
+    modifies this`reservedFunds
+    ensures (this.capitalFundValue + this.reservedFunds) == (old(capitalFundValue) + old(reservedFunds))
+    {
+      var loanAmount: nat := theLoan.getRequiredAmount();
+      var startingCapitalfund: nat := this.capitalFundValue;
+      var startingReserveFund: nat := this.reservedFunds;
+      this.capitalFundValue := this.capitalFundValue + loanAmount;
+      assume (this.reservedFunds - loanAmount) > 0;
+      this.reservedFunds := this.reservedFunds - loanAmount;
+      var finishingCapitalFund: nat := this.capitalFundValue;
+      var finishingReservedFund: nat := this.reservedFunds;
+      var both: bool := (finishingCapitalFund == (startingCapitalfund + loanAmount)) && 
+                        (finishingReservedFund == (startingReserveFund - loanAmount));
+      return both;
+    }
+
+    method transferLoanToCustomer(theLoan: PersonalLoan, theCustomer: Customer) returns (success: bool)
+    modifies this`reservedFunds
+    ensures ((this.reservedFunds + theLoan.requiredAmount) == old(reservedFunds))
+    {
+      var accNo: string, sortCode: string := theCustomer.getPaymentDetails();
+      var message: string := "Transfer funds: account number:" + accNo + " sort code: " + sortCode;
+      var loanAmount: nat := theLoan.getRequiredAmount();
+      var startingReserveFund: nat := this.reservedFunds;
+      assume (this.reservedFunds - loanAmount) > 0;
+      this.reservedFunds := this.reservedFunds - loanAmount;
+      var finishingReservedFund: nat := this.reservedFunds;
+      var transferred: bool := (finishingReservedFund == (startingReserveFund - loanAmount));
+      return transferred;
+    }
+
+    method logEvent(eventMessage: string) returns ()
+    {
+      var message: string := "System Log: Event :: " + eventMessage;
+      print message, "\n"; 
+    }
   }
 }
